prove adequacy for never_stuck

theories/lang/defs.v
@@ -84,6 +84,8 @@ Notation "x ~{ fn }~>+ y" := (tc (tstep fn) x y)
   (at level 70, format "x  ~{ fn }~>+  y").
 
 Definition reducible fs e σ := (∃ e' σ', (e,σ) ~{fs}~> (e', σ')).
+Definition never_stuck fs e σ :=
+  ∀ e' σ', (e, σ) ~{fs}~>* (e', σ') → terminal e' ∨ reducible fs  e' σ'.
 
 (*=================================== UNUSED =================================*)
 (* Implicit Type (ρ: cfg bor_lang). *)
