theories/sim/global_adequacy.v
@@ -1,7 +1,7 @@
 From Coq Require Import Program.Equality Lia.
 From Paco Require Import paco.
 
-From stbor.lang Require Import steps_wf.
+From stbor.lang Require Import steps_wf steps_inversion.
 From stbor.sim Require Import behavior global invariant sflib.
 
 Set Default Proof Using "Type".
@@ -29,7 +29,7 @@ Proof.
   - i. apply lt_le_S in H. inv H; eauto.
 Qed.
 
-Lemma stuck_terminal prog (eσ: expr * state):
+(* Lemma stuck_terminal prog (eσ: expr * state):
   stuck (Λ:=bor_lang prog) eσ.1 eσ.2 ↔ (∀ r, ¬ term prog eσ r) ∧ ∀ eσ', ¬ eσ ~{prog}~> eσ'.
 Proof.
  split => [[NT NS]|[NT NS]]; split.
@@ -39,40 +39,40 @@ Proof.
    apply (NT v Eqv).
  - intros ???? PRIM. apply (NS (e', σ')). by econstructor; eauto.
 Qed.
+ *)
 
-Lemma adequacy
-      prog_src `{NSD: Decision (∀ e σ, never_stuck prog_src e σ)}
+Lemma adequacy_never_stuck
+      prog_src
       prog_tgt idx conf_src conf_tgt
       (SIM: sim prog_src prog_tgt idx conf_src conf_tgt)
+      (WFS: Wf conf_src.2) (WFT: Wf conf_tgt.2)
+      (NEVERSTUCK: never_stuck prog_src conf_src.1 conf_src.2)
   : behave tstep term prog_tgt conf_tgt <1= behave tstep term prog_src conf_src.
 Proof.
-  revert idx conf_src conf_tgt SIM. pcofix CIH. intros.
+  revert idx conf_src conf_tgt SIM WFS WFT NEVERSTUCK. pcofix CIH. intros.
   punfold PR. inv PR.
-  rename x2 into obs. rename s' into conf'_tgt. revert idx conf_src SIM MAT.
+  rename x2 into obs. rename s' into conf'_tgt. revert idx conf_src WFS NEVERSTUCK SIM MAT.
   dependent induction TAU; cycle 1.
   - rename x into conf_tgt.
     rename y into conf'_tgt.
     rename z into conf''_tgt.
-    i. punfold SIM. exploit SIM.
-    { admit. (* never_stuck *) }
-    { admit. (* WF *) }
-    { admit. (* WF *) }
+    i. punfold SIM. exploit SIM; auto.
     clear SIM. intro SIM. inv SIM.
+    have WFT': Wf conf'_tgt.2 by eapply tstep_wf; eauto.
     exploit sim_step; eauto. i. revert sim_stuck. des.
     + inv x0; ss.
       rename eσ2_src into conf'_src.
-      exploit IHTAU; eauto.
+      have WFS' : Wf conf'_src.2 by eapply tstep_tc_wf; eauto.
+      exploit (IHTAU WFT' idx2 _ WFS'); eauto.
+      { eapply never_stuck_tstep_tc'; eauto. }
       intro BEH. punfold BEH. inv BEH.
       pfold. econs; [|by eauto]. etrans; eauto. apply tc_rtc. ss.
     + inv x0; ss.
       rename eσ2_src into conf'_src.
-      exploit IHTAU; eauto.
-  - intros idx. revert x.
+      exploit (IHTAU WFT' idx2 _ WFS); eauto.
+  - intros idx. revert x WFT.
     induction idx using strong_induction. i.
-    punfold SIM. exploit SIM.
-    { admit. (* never_stuck *) }
-    { admit. (* WF *) }
-    { admit. (* WF *) }
+    punfold SIM. exploit SIM; auto.
     clear SIM. intro SIM. inv SIM. inv MAT.
     + exfalso. destruct sim_stuck as [[v TE]|ST].
       * by apply (NT v).
@@ -85,12 +85,83 @@ Proof.
         { subst. reflexivity. }
       * unfold terminal in *. des.
         econs 2. unfold term. erewrite x2; eauto.
-    + pclearbot. exploit sim_step; eauto. i. revert sim_stuck. des.
+    + pclearbot. exploit sim_step; eauto. i. revert sim_stuck.
+      rename s' into conf'_tgt.
+      have WFT': Wf conf'_tgt.2 by eapply tstep_wf; eauto.
+      des.
       * inv x1; ss.
-        exploit CIH; eauto. intros ?.
+        rename eσ2_src into conf'_src.
+        exploit (CIH idx2 conf'_src conf'_tgt); eauto.
+        { by eapply tstep_tc_wf; eauto. }
+        { by eapply never_stuck_tstep_tc'; eauto. }
+        intros ?.
         apply tc_inv_l in x0. des.
         pfold. econs; eauto.
-      * inv x1; ss. exploit IH; eauto.
+      * inv x1; ss.
+        rename eσ2_src into conf'_src.
+        exploit (IH idx2 x0 conf'_tgt WFT' conf'_src); eauto.
+        punfold INF. inv INF. inv TAU; eauto.
+        econs 3; eauto.
+Qed.
+
+Lemma adequacy
+      prog_src `{NSD: ∀ e σ, Decision (never_stuck prog_src e σ)}
+      prog_tgt idx conf_src conf_tgt
+      (SIM: sim prog_src prog_tgt idx conf_src conf_tgt)
+      (WFS: Wf conf_src.2) (WFT: Wf conf_tgt.2)
+  : behave tstep term prog_tgt conf_tgt <1= behave tstep term prog_src conf_src.
+Proof.
+  revert idx conf_src conf_tgt SIM WFS WFT. pcofix CIH. intros.
+  punfold PR. inv PR.
+  rename x2 into obs. rename s' into conf'_tgt. revert idx conf_src WFS SIM MAT.
+  dependent induction TAU; cycle 1.
+  - rename x into conf_tgt.
+    rename y into conf'_tgt.
+    rename z into conf''_tgt.
+    i. punfold SIM. exploit SIM.
+    { admit. (* never_stuck *) }
+    clear SIM. intro SIM. inv SIM.
+    have WFT': Wf conf'_tgt.2 by eapply tstep_wf; eauto.
+    exploit sim_step; eauto. i. revert sim_stuck. des.
+    + inv x0; ss.
+      rename eσ2_src into conf'_src.
+      have WFS' : Wf conf'_src.2 by eapply tstep_tc_wf; eauto.
+      exploit (IHTAU WFT' idx2 _ WFS'); eauto.
+      intro BEH. punfold BEH. inv BEH.
+      pfold. econs; [|by eauto]. etrans; eauto. apply tc_rtc. ss.
+    + inv x0; ss.
+      rename eσ2_src into conf'_src.
+      exploit (IHTAU WFT' idx2 _ WFS); eauto.
+  - intros idx. revert x WFT.
+    induction idx using strong_induction. i.
+    punfold SIM. exploit SIM.
+    { admit. (* never_stuck *) }
+    clear SIM. intro SIM. inv SIM. inv MAT.
+    + exfalso. destruct sim_stuck as [[v TE]|ST].
+      * by apply (NT v).
+      * unfold reducible in ST. des. eapply NS.
+        destruct x. eauto.
+    + clear sim_stuck. exploit sim_terminal; eauto. i. des.
+      pfold. econs.
+      * instantiate (1 := eσ2_src). unguardH x0. des.
+        { apply tc_rtc. eauto. }
+        { subst. reflexivity. }
+      * unfold terminal in *. des.
+        econs 2. unfold term. erewrite x2; eauto.
+    + pclearbot. exploit sim_step; eauto. i. revert sim_stuck.
+      rename s' into conf'_tgt.
+      have WFT': Wf conf'_tgt.2 by eapply tstep_wf; eauto.
+      des.
+      * inv x1; ss.
+        rename eσ2_src into conf'_src.
+        exploit (CIH idx2 conf'_src conf'_tgt); eauto.
+        { by eapply tstep_tc_wf; eauto. }
+        intros ?.
+        apply tc_inv_l in x0. des.
+        pfold. econs; eauto.
+      * inv x1; ss.
+        rename eσ2_src into conf'_src.
+        exploit (IH idx2 x0 conf'_tgt WFT' conf'_src); eauto.
         punfold INF. inv INF. inv TAU; eauto.
         econs 3; eauto.
 Admitted.
